Migrate Inference and Proof to Clause
Now we don't have the problems with substitutions on formulas being unsound. Coercion from clauses to formulas works and everything can still be used.

InferenceInLean/Basic.lean
@@ -43,6 +43,7 @@ lemma Term.induction {sig : Signature} {X : Variables} {P : (Term sig X) → Pro
       intro term' harg'
       exact ih term' harg'
 
+@[simp]
 def Term.freeVars {sig : Signature} {X : Variables} : @Term sig X -> Set X
   | .var x => {x}
   | .func _ [] => ∅
@@ -53,6 +54,7 @@ inductive Atom (sig : Signature) (X : Variables) where
   | pred (p : sig.preds) (args : List (Term sig X))
   | eq (lhs rhs : Term sig X)
 
+@[simp]
 def Atom.freeVars {sig : Signature} {X : Variables} : @Atom sig X -> Set X
   | .pred _ args => args.foldl (fun acc t => acc ∪ Term.freeVars t) ∅
   | .eq lhs rhs => Term.freeVars lhs ∪ Term.freeVars rhs
@@ -61,10 +63,12 @@ inductive Literal (sig : Signature) (X : Variables) where
   | pos (a : @Atom sig X)
   | neg (a : @Atom sig X)
 
+@[simp]
 def Literal.comp {sig : Signature} {X : Variables} : Literal sig X -> Literal sig X
   | .pos a => .neg a
   | .neg a => .pos a
 
+@[simp]
 def Clause (sig : Signature) (X : Variables) := List (Literal sig X)
 
 instance {sig : Signature} {X : Variables} : Membership (Literal sig X) (Clause sig X) :=
@@ -81,6 +85,18 @@ inductive Formula (sig: Signature) (X: Variables) where
   | iff (f g : @Formula sig X)
   | all (x : X) (f : @Formula sig X)
   | ex (x : X) (f : @Formula sig X)
+
+@[simp]
+def Clause.toFormula {sig : Signature} {X : Variables} : @Clause sig X -> @Formula sig X
+  | [] => Formula.verum
+  | .pos l :: ls => Formula.or (Formula.atom l) (Clause.toFormula ls)
+  | .neg l :: ls => Formula.or (Formula.neg (Formula.atom l)) (Clause.toFormula ls)
+
+instance {sig : Signature} {X : Variables} : Coe (Clause sig X) (Formula sig X) :=
+  ⟨Clause.toFormula⟩
+
+instance {sig : Signature} {X : Variables} : Coe (Set <| Clause sig X) (Set <| Formula sig X) :=
+  ⟨fun N => {Clause.toFormula C | C ∈ N}⟩
 
 @[simp]
 def Substitution (sig : Signature) (X : Variables) := X -> Term sig X
@@ -115,6 +131,7 @@ infix:50 " ≤ " => MoreGeneral
 
 def example_subst : Substitution (Signature.mk String String) String :=
   fun x => if x == "z" then Term.func "f" [Term.var "y"] else Term.var x
+
 def example_subst' : Substitution (Signature.mk String String) String :=
   fun x => if x == "z" then Term.func "f" [Term.var "z"] else
     if x == "y" then Term.var "z" else Term.var x
@@ -125,6 +142,7 @@ theorem example_more_general : example_subst ≤ example_subst' := by
   simp [example_subst, example_subst']
   by_cases hx : x = "z" <;> by_cases hy : x = "y" <;> simp [hx, hy]
 
+@[simp]
 def Idempotent {sig : Signature} {X : Variables} [BEq X] (σ : Substitution sig X) : Prop :=
   σ ∘ σ = σ
 
@@ -195,6 +213,7 @@ def Assignment.modify_rfl {X : Variables} {univ : Universes} [DecidableEq X]
   · rfl
 
 -- x ≠ y → β[x ↦ a, y ↦ b] = β[y ↦ b, x ↦ a]
+@[simp]
 def Assignment.modify_comm {X : Variables} {univ : Universes} [DecidableEq X]
     {β : Assignment X univ} (x y : X) (a b : univ) :
     x ≠ y → (β.modify x a).modify y b = (β.modify y b).modify x a := by
@@ -205,7 +224,6 @@ def Term.eval {sig : Signature} {X : Variables}
     (I : Interpretation sig) (β : Assignment X I.univ) : @Term sig X -> I.univ
   | Term.var x => β x
   | Term.func f args => (I.functions f) <| args.attach.map (fun ⟨a, _⟩ => Term.eval I β a)
-
 
 @[simp]
 def Atom.substitute {sig : Signature} {X : Variables} [DecidableEq X]
@@ -245,29 +263,6 @@ def Formula.freeVars {sig : Signature} {X : Variables} : @Formula sig X -> Set X
   | Formula.iff f g => Formula.freeVars f ∪ Formula.freeVars g
   | Formula.all x f => Formula.freeVars f \ {x}
   | Formula.ex x f => Formula.freeVars f \ {x}
-
-
-/-
-TODO: take care of bound variables in quantifiers or maybe just dont care?
-(Qx F)σ = Qz (F σ[x → z]) with z a fresh variable and Q ∈ {∀, ∃}
-However, how can we cleanly ensure that z is fresh?
-Do we even need to? Let's not do it now and mabye add some hypothesis for the substiution later.
-This should force drastic modifications of everything buildng on this (fingers crossed).
--/
-@[simp]
-def Formula.substitute {sig : Signature} {X : Variables}
-    [inst : DecidableEq X] [inst_nonempty : Nonempty X]
-    (σ : Substitution sig X) : @Formula sig X -> @Formula sig X
-  | Formula.falsum => Formula.falsum
-  | Formula.verum => Formula.verum
-  | Formula.atom a => Formula.atom (Atom.substitute σ a)
-  | Formula.neg f => Formula.neg (substitute σ f)
-  | Formula.and f g => Formula.and (substitute σ f) (substitute σ g)
-  | Formula.or f g => Formula.or (substitute σ f) (substitute σ g)
-  | Formula.imp f g => Formula.imp (substitute σ f) (substitute σ g)
-  | Formula.iff f g => Formula.iff (substitute σ f) (substitute σ g)
-  | Formula.all x f => Formula.all x (substitute σ f)
-  | Formula.ex x f => Formula.all x (substitute σ f)
 
 
 /-
@@ -335,21 +330,73 @@ theorem entails_iff_and_not_unsat {sig : Signature} {X : Variables} [inst : Deci
     (F G : Formula sig X) :
     Entails F G ↔ @Unsatisfiable sig X inst (Formula.and F (Formula.neg G)) := by simp
 
-/-
-Expand this to sets of Formulas
--/
+@[simp]
+def Literal.satisfied_by {sig : Signature} {X: Variables} [DecidableEq X]
+    (L : Literal sig X) (I : @Interpretation sig) (β : Assignment X I.univ) : Prop :=
+  EntailsInterpret I β <| match L with
+    | Literal.pos a => Formula.atom a
+    | Literal.neg a => Formula.neg (Formula.atom a)
+
 @[simp]
 def SetEntails {sig : Signature} {X : Variables} [DecidableEq X]
     (N : Set (Formula sig X)) (F : Formula sig X) : Prop :=
   ∀ (I : @Interpretation sig) (β : Assignment X I.univ),
     (∀ G ∈ N, EntailsInterpret I β G) → EntailsInterpret I β F
 
+@[simp]
+def ClauseSetEntails {sig : Signature} {X : Variables} [DecidableEq X]
+    (N : Set <| Clause sig X) (C : Clause sig X) : Prop :=
+  ∀ (I : @Interpretation sig) (β : Assignment X I.univ),
+    (∀ D ∈ N, EntailsInterpret I β D) → EntailsInterpret I β C
+
 lemma entails_setEntails {sig : Signature} {X : Variables} [inst : DecidableEq X]
     (F G : Formula sig X) : Entails F G ↔ @SetEntails sig X inst {F} G := by simp
 
 @[simp]
+def ClauseSatisfiable {sig : Signature} {X : Variables} [DecidableEq X] (C : Clause sig X) : Prop :=
+  ∃ (I : @Interpretation sig) (β : Assignment X I.univ),
+    ∃ L : Literal sig X, L ∈ C ∧ L.satisfied_by I β
+
+@[simp]
+theorem ClauseSatisfiable_imp_Satisfiable {sig : Signature} {X : Variables} [inst : DecidableEq X]
+    (C : Clause sig X) : ClauseSatisfiable C → @Satisfiable sig X inst ↑C := by
+  simp only [ClauseSatisfiable, Assignment, Satisfiable, EntailsInterpret]
+  intro ⟨I, ⟨β, ⟨L, ⟨h_L_in_C, hsatby⟩⟩⟩⟩
+  use I, β
+  induction C with
+  | nil =>
+    exact False.elim (List.not_mem_nil L h_L_in_C)
+  | cons head Ctail ih =>
+    rw [Clause.toFormula.eq_def]
+    split
+    next => simp only [Formula.eval]
+    all_goals -- proof cases for Literal.pos and Literal.neg at once
+    next h_split atom tail h_head_pos_atom =>
+      simp_all only [List.cons.injEq, Formula.eval]
+      obtain ⟨h_head_atom, _⟩ := h_head_pos_atom
+      have mem_head : L = head ∨ L ∈ tail := by simp [h_head_atom, List.mem_cons.mp h_L_in_C]
+      cases mem_head
+      next _h_is_head =>
+        constructor
+        simp_all only [List.cons.injEq, true_and, Atom.eval]
+        exact hsatby
+      next h_in_tail =>
+        apply Or.inr
+        exact ih h_in_tail
+
+@[simp]
 def SetSatisfiable {sig : Signature} {X : Variables} [DecidableEq X]
     (N : Set (@Formula sig X)) : Prop :=
+  ∃ (I : @Interpretation sig) (β : Assignment X I.univ), ∀ G ∈ N, EntailsInterpret I β G
+
+@[simp]
+def ClauseSetSatisfiableByLiterals {sig : Signature} {X : Variables} [DecidableEq X]
+    (N : Set <| Clause sig X) : Prop :=
+  ∃ (I : @Interpretation sig) (β : Assignment X I.univ), ∀ C ∈ N, ∃ L ∈ C, L.satisfied_by I β
+
+@[simp]
+def ClauseSetSatisfiable {sig : Signature} {X : Variables} [DecidableEq X]
+    (N : Set <| Clause sig X) : Prop :=
   ∃ (I : @Interpretation sig) (β : Assignment X I.univ), ∀ G ∈ N, EntailsInterpret I β G
 
 @[simp]
@@ -368,26 +415,11 @@ lemma unsat_as_set_unsat {sig : Signature} {X : Variables} [inst : DecidableEq X
 theorem setEntails_iff_union_not_unsat {sig : Signature} {X : Variables} [inst : DecidableEq X]
     (N : Set $ Formula sig X) (G : Formula sig X) :
     SetEntails N G ↔ @SetUnsatisfiable sig X inst (N ∪ {Formula.neg G}) := by
-        sorry
+  sorry
 
-/-Expand this to Literals and Clauses-/
-def Literal.satisfied_by {sig : Signature} {X: Variables} [DecidableEq X]
-    (L : Literal sig X) (I : @Interpretation sig) (β : Assignment X I.univ) : Prop :=
-  EntailsInterpret I β <| match L with
-    | Literal.pos a => Formula.atom a
-    | Literal.neg a => Formula.neg (Formula.atom a)
-
-def ClauseSatisfiable {sig : Signature} {X : Variables} [DecidableEq X] (C : Clause sig X) : Prop :=
-  ∃ (I : @Interpretation sig) (β : Assignment X I.univ),
-    ∃ L : Literal sig X, L ∈ C ∧ L.satisfied_by I β
-
-def ClauseSetSatisfiable {sig : Signature} {X : Variables} [DecidableEq X]
-    (N : Set <| Clause sig X) : Prop :=
-  ∃ (I : @Interpretation sig) (β : Assignment X I.univ), ∀ C ∈ N, ∃ L, L ∈ C ∧ L.satisfied_by I β
 
 /-
 ### 3.3.4 Substitution Lemma
-- do it later maybe
 -/
 @[simp]
 def Assignment.compose {sig : Signature} {X : Variables} [DecidableEq X]
@@ -428,7 +460,6 @@ theorem substitution_lemma' {sig : Signature} {X : Variables} [DecidableEq X]
         List.map (Assignment.compose I β σ) args = .map (Term.eval I β ∘ .substitute σ) args := by
       simp_all only [List.map_inj_left, Function.comp_apply, implies_true]
     rw [hargsarequal]
-
 
 -- for variables x_1,...,x_n and formula F, this returns ∀ x_1 ... x_n, F
 @[simp]
@@ -731,6 +762,7 @@ def EqualityProblem (sig : Signature) (X : Variables) :=
 instance {sig : Signature} {X : Variables} : Membership (Equality sig X) (EqualityProblem sig X) :=
   List.instMembership
 
+@[simp]
 def EqualityProblem.freeVars {sig : Signature} {X : Variables} :
     @EqualityProblem sig X -> Set X
   | [] => ∅
@@ -766,7 +798,7 @@ theorem unifiable_iff_mgu_idempot {sig : Signature} {X : Variables} [inst : Deci
     (E : EqualityProblem sig X) : Unifiable E ↔ ∃ σ : Substitution sig X,
       MostGeneralUnifier E σ ∧ Idempotent σ ∧ σ.domain ∪ σ.codomain ⊆ E.freeVars := by
   apply Iff.intro
-  · sorry
+  · sorry -- this will need the standard unification algorithm
   · intro h
     obtain ⟨σ, ⟨⟨⟩⟩⟩ := h
     use σ
@@ -776,49 +808,54 @@ alias main_unification_theorem := unifiable_iff_mgu_idempot
 /-
 ### 3.7 Inference Systems and Proofs
 -/
-structure Inference (sig : Signature) (X : Variables) where
-  premises : Set (Formula sig X)
-  conclusion : Formula sig X
 
--- TODO: make this def := List
-structure InferenceSystem (sig : Signature) (X : Variables) where
-  inferences : List (Inference sig X)
+/--
+We limit this to clausal proofs.
+-/
+structure Inference (sig : Signature) (X : Variables) where
+  premises : Set (Clause sig X)
+  conclusion : Clause sig X
+
+def InferenceSystem (sig : Signature) (X : Variables) := List (Inference sig X)
+
+instance {sig : Signature} {X : Variables} : Membership (Inference sig X) (InferenceSystem sig X) :=
+  List.instMembership
 
 structure Proof {sig : Signature} {X : Variables} (Γ : InferenceSystem sig X) where
-  assumptions : Set (Formula sig X)
-  conclusion : Formula sig X
-  formulas : List (Formula sig X)
-  formulas_not_empty : formulas ≠ ∅
-  last_formula_conclusion : formulas[formulas.length - 1]'(by
-    have hlennonzero : formulas.length ≠ 0 := by
+  assumptions : Set (Clause sig X)
+  conclusion : Clause sig X
+  clauses : List (Clause sig X)
+  clauses_not_empty : clauses ≠ ∅
+  last_clause_conclusion : clauses[clauses.length - 1]'(by
+    have hlennonzero : clauses.length ≠ 0 := by
       simp_all only [List.empty_eq, ne_eq, List.length_eq_zero, not_false_eq_true]
     exact Nat.sub_one_lt hlennonzero) = conclusion
-  is_valid : ∀ i (hindex : i < formulas.length), formulas[i] ∈ assumptions ∨
-    ∃ inference ∈ Γ.inferences, formulas[i] = inference.conclusion ∧
-      ∀ formula ∈ inference.premises, ∃ (j : ℕ) (hjindex : j < i), formula = formulas[j]
+  is_valid : ∀ i (hindex : i < clauses.length), clauses[i] ∈ assumptions ∨
+    ∃ inference ∈ Γ, clauses[i] = inference.conclusion ∧
+      ∀ Clause ∈ inference.premises, ∃ (j : ℕ) (hjindex : j < i), Clause = clauses[j]
 
 @[simp]
 def Provability {sig : Signature} {X : Variables}
-    (Γ : InferenceSystem sig X) (N : Set (Formula sig X)) (F : Formula sig X) : Prop :=
+    (Γ : InferenceSystem sig X) (N : Set (Clause sig X)) (F : Clause sig X) : Prop :=
   ∃ proof : Proof Γ, proof.assumptions = N ∧ proof.conclusion = F
 
 @[simp]
 def Soundness {sig : Signature} {X : Variables} [inst : DecidableEq X]
     (Γ : InferenceSystem sig X) : Prop :=
-  ∀ inference ∈ Γ.inferences, SetEntails inference.premises inference.conclusion
+  ∀ inference ∈ Γ, ClauseSetEntails inference.premises inference.conclusion
 
 @[simp]
 def GeneralSoundness {sig : Signature} {X : Variables} [inst : DecidableEq X]
     (Γ : InferenceSystem sig X) : Prop :=
-  ∀ (N : Set (Formula sig X)) (F : Formula sig X), Provability Γ N F → SetEntails N F
+  ∀ (N : Set (Clause sig X)) (F : Clause sig X), Provability Γ N F → ClauseSetEntails N F
 
 theorem generalSoundness_of_soundness {sig : Signature} {X : Variables} [inst : DecidableEq X]
     (Γ : InferenceSystem sig X) : Soundness Γ → GeneralSoundness Γ := by
   intro hsound N F hproof A β hgstrue
   rcases hproof with ⟨proof, ⟨hassumptions, hconclusion⟩⟩
-  have hproofsequencetrue : ∀ F ∈ proof.formulas, EntailsInterpret A β F := by
-    have hindicestrue : ∀ i (hindex : i < proof.formulas.length),
-        EntailsInterpret A β proof.formulas[i] := by
+  have hproofsequencetrue : ∀ F ∈ proof.clauses, EntailsInterpret A β F := by
+    have hindicestrue : ∀ i (hindex : i < proof.clauses.length),
+        EntailsInterpret A β proof.clauses[i] := by
       intro i hlen
       induction' i using Nat.case_strong_induction_on with i ih
       · have hvalid := proof.is_valid 0 hlen
@@ -837,17 +874,17 @@ theorem generalSoundness_of_soundness {sig : Signature} {X : Variables} [inst : 
           rw [heq]
           exact hjtrue
     intro F hF
-    have hfindex : ∃ (i : ℕ) (hindex : i < proof.formulas.length), proof.formulas[i] = F :=
+    have hfindex : ∃ (i : ℕ) (hindex : i < proof.clauses.length), proof.clauses[i] = F :=
       List.mem_iff_getElem.mp hF
     aesop
-  have hlen : proof.formulas.length - 1 < proof.formulas.length := by
-    have hlennonzero : proof.formulas.length ≠ 0 := by
-      have hnonempty := proof.formulas_not_empty
+  have hlen : proof.clauses.length - 1 < proof.clauses.length := by
+    have hlennonzero : proof.clauses.length ≠ 0 := by
+      have hnonempty := proof.clauses_not_empty
       simp_all only [List.empty_eq, ne_eq, List.length_eq_zero, not_false_eq_true]
     exact Nat.sub_one_lt hlennonzero
-  have hfconclusion := proof.is_valid (proof.formulas.length - 1) hlen
-  have hfislast : proof.formulas[proof.formulas.length - 1] = F := by
-    rw [proof.last_formula_conclusion, hconclusion]
+  have hfconclusion := proof.is_valid (proof.clauses.length - 1) hlen
+  have hfislast : proof.clauses[proof.clauses.length - 1] = F := by
+    rw [proof.last_clause_conclusion, hconclusion]
   rw [hfislast] at hfconclusion
   rcases hfconclusion with hl | hr
   · simp_all only [Soundness, SetEntails, Assignment, EntailsInterpret]
@@ -868,40 +905,64 @@ theorem generalSoundness_of_soundness {sig : Signature} {X : Variables} [inst : 
 ### 3.8 Ground (or Propositional) Resolution
 -/
 
-theorem groundResolution_soundness {sig : Signature} {X : Variables} {D A C : Formula sig X}
-    [inst : DecidableEq X] (Resolution : Inference sig X)
-    (hresolution : Resolution = ⟨{.or D A, .or C (.neg A)}, .or D C⟩)
-    (Factorization : Inference sig X)
-    (hfactorization : Factorization = ⟨{.or (.or C A) A}, .or C A⟩)
-    (Γ_Resolution : InferenceSystem sig X) (hgamma : Γ_Resolution = ⟨[Resolution, Factorization]⟩) :
-    Soundness Γ_Resolution := by
-  intro inference hinf I β hgstrue
-  -- aesop would already close the goal here
-  subst hresolution hgamma hfactorization
-  simp_all only [EntailsInterpret, List.mem_cons, List.mem_singleton, List.not_mem_nil, or_false]
-  rcases hinf with hres | hfact
-  -- we first show that the resolution inference rule is correct
-  · subst hres
-    simp_all only [Set.mem_insert_iff, Set.mem_singleton_iff,
-      forall_eq_or_imp, Formula.eval, forall_eq]
-    obtain ⟨D_or_A, C_or_notA⟩ := hgstrue
-    rcases D_or_A with hD | hA
-    · left
-      exact hD
-    · rcases C_or_notA with hC | hnA
-      · right
-        exact hC
-      · exact False.elim (hnA hA)
-  -- next, we show that the factorization inference rule is correct
-  · subst hfact
-    simp_all only [Set.mem_singleton_iff, Formula.eval, forall_eq]
-    rcases hgstrue with (hC | hA) | hA
-    · left
-      exact hC
-    · right
-      exact hA
-    · right
-      exact hA
+@[simp]
+def FactorizationRule {sig : Signature} (A : Atom sig Empty) (C : Clause sig Empty) :
+    Inference sig Empty :=
+  ⟨{.pos A :: .pos A :: C}, .pos A :: C⟩
+
+@[simp]
+def ResolutionRule {sig : Signature} (A : Atom sig Empty) (C D : Clause sig Empty) :
+    Inference sig Empty :=
+  ⟨{.pos A :: C, .neg A :: D}, C.append D⟩
+
+/--
+Both rules of the Resolution Calculus.
+Note that at the moment this is an inference system.
+Ideally we could somehow move the `A C D` inside the rules to use factorization without `D`.
+-/
+@[simp]
+def GroundResolution (sig : Signature) (A : Atom sig Empty) (C D : Clause sig Empty) :
+    InferenceSystem sig Empty :=
+  [ResolutionRule A C D, FactorizationRule A C]
+
+lemma ground_clause_iff_literal {sig: Signature}
+    (I : Interpretation sig) (β : Assignment Empty I.univ) (C : Clause sig Empty) :
+    Formula.eval I β ↑C ↔ (∃ L ∈ C, L.satisfied_by I β) ∨ C = [] := by
+  apply Iff.intro
+  · intro h_eval
+    induction C with
+    | nil => simp
+    | cons head tail ih =>
+      left
+      by_cases hl : head.satisfied_by I β
+      · use head
+        simp_all only [Clause, Literal.satisfied_by, EntailsInterpret, List.mem_cons, true_or,
+          and_self]
+      · sorry -- show that ¬head.sat ∨ .eval ↑(head :: tail) → .eval ↑tail using `false_or`
+  · sorry -- this should be the easier case using induction on C and `List.mem_cons`
+
+
+theorem groundResolution_soundness {sig : Signature }
+    {A : Atom sig Empty} {C D : Clause sig Empty} : Soundness (GroundResolution sig A C D):= by
+  rw [Soundness]
+  intro rule h_rule_ground I β h_premise_true
+  simp [EntailsInterpret]
+  simp_all only [GroundResolution, ResolutionRule, Clause, List.append_eq, FactorizationRule,
+    EntailsInterpret]
+  rw [List.mem_cons, List.mem_singleton] at h_rule_ground
+  cases h_rule_ground
+  -- proof of resolution rule
+  next h_res_rule =>
+    subst h_res_rule
+    simp_all only [Set.mem_insert_iff, Set.mem_singleton_iff, forall_eq_or_imp, forall_eq]
+    obtain ⟨h_posAconsC, h_negAconsD⟩ := h_premise_true
+    have := (ground_clause_iff_literal I β (Literal.pos A :: C)).mp h_posAconsC
+    sorry -- the heavy lifting here should be done by `ground_clause_iff_literal`
+  -- proof of factorization rule
+  next h_fact_rule =>
+    subst h_fact_rule
+    simp_all only [Clause, Set.mem_singleton_iff, Clause.toFormula, Formula.eval, Atom.eval,
+      or_self_left, forall_eq]
 
 /-
 ## Further stuff:
